theories/simulang/na_inv/examples/derived.v
@@ -1,0 +1,22 @@
+From iris Require Import bi.bi.
+From iris.proofmode Require Import tactics.
+From simuliris.simulation Require Import slsls lifting.
+From simuliris.simulang Require Import lang notation tactics
+  proofmode log_rel_structural wf behavior.
+From simuliris.simulang.na_inv Require Export inv.
+From simuliris.simulang.na_inv Require Import readonly_refl adequacy.
+From iris.prelude Require Import options.
+
+(** * Derived stuff we show in the paper *)
+
+Section derived.
+  Context `{naGS Σ}.
+
+
+  Lemma safe_reach_if e1 e2 v : safe_reach (∃ b, v = LitV $ LitBool b) (If (Val v) e1 e2).
+  Proof. apply safe_reach_irred. apply _. Qed.
+  Lemma safe_reach_div v1 v2 : safe_reach ((∃ n, v1 = LitV $ LitInt n) ∧ (∃ n, v2 = LitV $ LitInt n ∧ n ≠ 0%Z))%V (BinOp QuotOp (Val v1) (Val v2)).
+  Proof. apply safe_reach_irred. apply _. Qed.
+  Lemma safe_reach_load o v_l : safe_reach (∃ l, v_l = LitV $ LitLoc l) (Load o $ Val v_l).
+  Proof. apply safe_reach_irred. apply _. Qed.
+End derived.
